@base          <http://www.w3.org/ns/auth/acl> .
@prefix :      <#> .
@prefix dc:    <http://purl.org/dc/elements/1.1/> .
@prefix rdf:   <http://www.w3.org/1999/02/22-rdf-syntax-ns#> .
@prefix rdfs:  <http://www.w3.org/2000/01/rdf-schema#> .

<http://www.w3.org/ns/auth/acl>
        dc:title      "Basic Access Control ontology" ;
        rdfs:comment  "Defines the class Authorization and its essential properties,\n    and also some classes of access such as read and write. " .

:Access a      rdfs:Class ;
        rdfs:comment  "Any kind of access to a resource. Don't use this, use R W and RW" ;
        rdfs:label  "access"@en .

:Append  a        rdfs:Class ;
        rdfs:comment     "Append accesses are specific write access which only add information, and do not remove information.\n    For text files, for example, append access allows bytes to be added onto the end of the file.\n    For RDF graphs, Append access allows adds triples to the graph but does not remove any.\n    Append access is useful for dropbox functionality.\n    Dropbox can be used for link notification, which the information added is a notification\n    that a some link has been made elsewhere relevant to the given resource.\n    " ;
        rdfs:label       "append"@en ;
        rdfs:subClassOf  :Access ;
        rdfs:subClassOf  :Write .

:AuthenticatedAgent  a  rdfs:Class ;
        rdfs:comment     "A class of agents who have been authenticated.\nIn other words, anyone can access this resource, but not anonymously.\nThe social expectation is that the authentication process will provide an\nidentify and a name, or pseudonym.\n(A new ID should not be minted for every access: the intent is that the user\nis able to continue to use the ID for continues interactions with peers,\nand for example to develop a reputation)\n" ;
        rdfs:label       "Anyone authenticated" ;
        rdfs:subClassOf  <http://xmlns.com/foaf/0.1/Agent> .

:Authorization  a  rdfs:Class ;
        rdfs:comment  "An element of access control,\n    allowing agent to agents access of some kind to resources or classes of resources" ;
        rdfs:label    "authorization" .

:Control  a       rdfs:Class ;
        rdfs:comment     "Allows read/write access to the ACL for the resource(s)" ;
        rdfs:label       "control"@en ;
        rdfs:subClassOf  :Access .

:Read   a         rdfs:Class ;
        rdfs:comment     "The class of read operations" ;
        rdfs:label       "read"@en ;
        rdfs:subClassOf  :Access .

:Write  a         rdfs:Class ;
        rdfs:label       "write"@en ;
        rdfs:subClassOf  :Access .

:accessControl  a    rdf:Property ;
        rdfs:comment        "The Access Control file for this information resource.\n        This may of course be a virtual resorce implemented by the access control system.\n        Note also HTTP's header  Link:  foo.meta ;rel=meta can be used for this." ;
        rdfs:domain         <http://www.w3.org/2006/gen/ont#InformationResource> ;
        rdfs:label          "access control" ;
        rdfs:range          <http://www.w3.org/2006/gen/ont#InformationResource> ;
        rdfs:subPropertyOf  rdfs:seeAlso .

:accessTo  a   rdf:Property ;
        rdfs:comment  "The information resource to which access is being granted." ;
        rdfs:domain   :Authorization ;
        rdfs:label    "to" ;
        rdfs:range    <http://www.w3.org/2006/gen/ont#InformationResource> .

:accessToClass  a  rdf:Property ;
        rdfs:comment  "A class of information resources to which access is being granted." ;
        rdfs:domain   :Authorization ;
        rdfs:label    "to all in" ;
        rdfs:range    rdfs:Class .

:agent  a      rdf:Property ;
        rdfs:comment  "A person or social entity to being given the right" ;
        rdfs:domain   :Authorization ;
        rdfs:label    "agent" ;
        rdfs:range    <http://xmlns.com/foaf/0.1/Agent> .

:agentClass  a  rdf:Property ;
        rdfs:comment  "A class of persons or social entities to being given the right" ;
        rdfs:domain   :Authorization ;
        rdfs:label    "agent class" ;
        rdfs:range    rdfs:Class .

:agentGroup  a  rdf:Property ;
        rdfs:comment  "A group of persons or social entities to being given the right" ;
        rdfs:domain   :Authorization ;
        rdfs:label    "agent group" ;
        rdfs:range    <http://www.w3.org/2006/vcard/ns#Group> .

:default  a    rdf:Property ;
        rdfs:comment  "A directory for which this authorization is used for new files in the directory." ;
        rdfs:domain   :Authorization ;
        rdfs:label    "default access for things in this" .

:defaultForNew  a  rdf:Property ;
        rdfs:comment  "THIS IS OBSOLETE AS OF 2017-08-01.   See 'default'.\n        Was: A directory for which this authorization is used for new files in the directory." ;
        rdfs:domain   :Authorization ;
        rdfs:label    "default access for new things in the object" .

:delegates  a  rdf:Property ;
        rdfs:comment  "Delegates a person or another agent to act on behalf of the agent.\n    For example, Alice delegates Bob to act on behalf of Alice for ACL purposes." ;
        rdfs:label    "delegates"@en ;
        rdfs:range    <http://xmlns.com/foaf/0.1/Agent> .

:mode   a      rdf:Property ;
        rdfs:comment  "A mode of access such as read or write." ;
        rdfs:domain   :Authorization ;
        rdfs:label    "access mode" ;
        rdfs:range    rdfs:Class .

:owner  a      rdf:Property ;
        rdfs:comment  "The person or other agent which owns this.\n    For example, the owner of a file in a filesystem.\n    There is a sense of right to control.   Typically defaults to the agent who craeted\n    something but can be changed." ;
        rdfs:label    "owner"@en ;
        rdfs:range    <http://xmlns.com/foaf/0.1/Agent> .

<https://www.w3.org/wiki/WebAccessControl>
        dc:describes  <http://www.w3.org/ns/auth/acl> .
