@base           <https://w3id.org/atomgraph/linkeddatahub/apps> .

@prefix :	<#> .
@prefix ldh:	<https://w3id.org/atomgraph/linkeddatahub#> .
@prefix a:	<https://w3id.org/atomgraph/core#> .
@prefix rdf:	<http://www.w3.org/1999/02/22-rdf-syntax-ns#> .
@prefix rdfs:	<http://www.w3.org/2000/01/rdf-schema#> .
@prefix xsd:	<http://www.w3.org/2001/XMLSchema#> .
@prefix owl:	<http://www.w3.org/2002/07/owl#> .
@prefix ldt:	<https://www.w3.org/ns/ldt#> .
@prefix sp:	<http://spinrdf.org/sp#> .
@prefix spin:	<http://spinrdf.org/spin#> .
@prefix spl:	<http://spinrdf.org/spl#> .
@prefix void:	<http://rdfs.org/ns/void#> .
@prefix foaf:	<http://xmlns.com/foaf/0.1/> .
@prefix dct:	<http://purl.org/dc/terms/> .

: a owl:Ontology ;
    owl:imports ldh:, ldt:, sp:, spin: ;
    rdfs:label "LinkedDataHub application ontology" ;
    rdfs:comment "Ontology of LinkedDataHub applications" ;
    owl:versionInfo "1.1.4" .

# PROPERTIES

:adminApplication a owl:ObjectProperty, owl:FunctionalProperty, owl:InverseFunctionalProperty ;
    owl:inverseOf :endUserApplication ;
    rdfs:domain :EndUserApplication ;
    rdfs:range :AdminApplication ;
    rdfs:label "Admin application" ;
    rdfs:comment "Links end-user application to its administration application" ;
    rdfs:isDefinedBy : .

:endUserApplication a owl:ObjectProperty, owl:FunctionalProperty, owl:InverseFunctionalProperty ;
    owl:inverseOf :adminApplication ;
    rdfs:domain :AdminApplication ;
    rdfs:range :EndUserApplication ;
    rdfs:label "End-user application" ;
    rdfs:comment "Links administration application to its end-user application" ;
    rdfs:isDefinedBy : .

:frontendProxy a owl:ObjectProperty ;
    rdfs:domain :Dataset ;
    rdfs:range rdfs:Resource ;
    rdfs:label "Frontend proxy" ;
    rdfs:comment "An intermediary server (such as cache) that proxies frontend requests to service" ;
    rdfs:isDefinedBy : .

:backendProxy a owl:ObjectProperty ;
    rdfs:domain :Dataset ;
    rdfs:range rdfs:Resource ;
    rdfs:label "Backend proxy" ;
    rdfs:comment "An intermediary server (such as cache) that proxies backend requests to service" ;
    rdfs:isDefinedBy : .

:public a owl:DatatypeProperty ;
    rdfs:domain :EndUserApplication ;
    rdfs:range xsd:boolean ;
    rdfs:label "Public" ;
    rdfs:comment "If true, this application can be listed as public (ACL still applies). If false, it is private and will not be listed" ;
    rdfs:isDefinedBy : .

:allowRead a owl:DatatypeProperty ;
    rdfs:domain :Application ;
    rdfs:range xsd:boolean ;
    rdfs:label "Allow read" ;
    rdfs:comment "If true, this application allows GET an HEAD methods for all request URIs without authorization check" ;
    rdfs:isDefinedBy : .

# CLASSES

# dataset

:Dataset a rdfs:Class, owl:Class ;
    rdfs:subClassOf void:Dataset ;
    rdfs:label "Linked Data dataset" ;
    rdfs:comment "A dataspace that returns RDF Linked Data" ;
    rdfs:isDefinedBy : .

# application

:Application a rdfs:Class, owl:Class ;
    rdfs:subClassOf ldt:Application ;
    spin:constructor :ApplicationConstructor ;
    spin:constraint :StartsWithHTTPS, :ValidOrigin,
        [ a ldh:MissingPropertyValue ;
            rdfs:label "Missing origin URI" ;
            sp:arg1 :origin
        ] ;
    rdfs:label "Application" ;
    rdfs:comment "An application represents a data space identified by its origin URI, in which application resource URIs are relative to the origin URI. The only application interface (API) is read-write RESTful Linked data, backed by an RDF dataset accessible as a SPARQL 1.1 service. Application structure is defined in an ontology, which can import other ontologies." ;
    rdfs:isDefinedBy : .

:ApplicationConstructor a ldh:Constructor ;
    sp:text """
      PREFIX lapp:    <https://w3id.org/atomgraph/linkeddatahub/apps#>
      PREFIX rdfs:    <http://www.w3.org/2000/01/rdf-schema#>

      CONSTRUCT {
          $this lapp:origin [ a rdfs:Resource ] .
      }
      WHERE {
    }""" ;
    rdfs:label "Application constructor" ;
    rdfs:isDefinedBy : .

# end-user

:EndUserApplication a rdfs:Class, owl:Class ;
    spin:constructor :EndUserApplicationConstructor ;
    spin:constraint [ a ldh:MissingPropertyValue ;
            rdfs:label "Missing admin application" ;
            sp:arg1 :adminApplication
        ] ;
    rdfs:label "End-user application" ;
    rdfs:comment "Application with a dynamic access control and sitemap" ;
    rdfs:isDefinedBy : .

:EndUserApplicationConstructor a ldh:Constructor ;
    sp:text """
      PREFIX lapp:    <https://w3id.org/atomgraph/linkeddatahub/apps#>
      PREFIX ldh:     <https://w3id.org/atomgraph/linkeddatahub#>
      PREFIX ac:      <https://w3id.org/atomgraph/client#>
      PREFIX xsd:     <http://www.w3.org/2001/XMLSchema#>
      PREFIX ldt:     <https://www.w3.org/ns/ldt#>
      PREFIX dct:     <http://purl.org/dc/terms/>

      CONSTRUCT {
          $this dct:title [ a xsd:string ] ;
            dct:description [ a xsd:string ] ;
            lapp:adminApplication [ a lapp:AdminApplication ] ;
            ac:stylesheet [ a ldh:File ] ;
            lapp:public [ a xsd:boolean ] .
      }
      WHERE {}""" ;
    rdfs:label "End-user application constructor" ;
    rdfs:isDefinedBy : .

# admin

:AdminApplication a rdfs:Class, owl:Class ;
    spin:constructor :AdminApplicationConstructor ;
    spin:constraint [ a ldh:MissingPropertyValue ;
            rdfs:label "Missing end-user application" ;
            sp:arg1 :endUserApplication
        ] ;
    rdfs:label "Admin application" ;
    rdfs:comment "Meta-application that manages the access control and sitemap of the main end-user application" ;
    rdfs:isDefinedBy : .

:AdminApplicationConstructor a ldh:Constructor ;
    sp:text """
      PREFIX lapp:    <https://w3id.org/atomgraph/linkeddatahub/apps#>
      PREFIX xsd:     <http://www.w3.org/2001/XMLSchema#>
      PREFIX dct:     <http://purl.org/dc/terms/>

      CONSTRUCT {
          $this dct:title [ a xsd:string ] ;
            dct:description [ a xsd:string ] ;
            lapp:endUserApplication [ a lapp:EndUserApplication ] ;
      }
      WHERE {}""" ;
    rdfs:label "Admin application constructor" ;
    rdfs:isDefinedBy : .

# CONSTRAINTS

:StartsWithHTTPS a sp:Construct ;
    rdfs:label "lapp:origin starts with https://" ;
    sp:text """
PREFIX  lapp: <https://w3id.org/atomgraph/linkeddatahub/apps#>
PREFIX  spin: <http://spinrdf.org/spin#>
PREFIX  rdfs: <http://www.w3.org/2000/01/rdf-schema#>

CONSTRUCT {
    _:c0 a spin:ConstraintViolation .
    _:c0 spin:violationRoot ?this .
    _:c0 spin:violationPath lapp:origin .
    _:c0 rdfs:label "Application origin URI must start with https://" .
}
WHERE {
  ?this  lapp:origin  ?origin
  FILTER ( ! strstarts(str(?origin), "https://") )
}""" ;
    rdfs:isDefinedBy : .

:ValidOrigin a sp:Construct ;
    rdfs:label "Origin must not have trailing slash and must have hostname" ;
    sp:text """
PREFIX  lapp: <https://w3id.org/atomgraph/linkeddatahub/apps#>
PREFIX  spin: <http://spinrdf.org/spin#>
PREFIX  rdfs: <http://www.w3.org/2000/01/rdf-schema#>

CONSTRUCT 
  { 
    _:c0 a spin:ConstraintViolation .
    _:c0 spin:violationRoot ?this .
    _:c0 spin:violationPath lapp:origin .
    _:c0 rdfs:label ?message .
  }
WHERE
  { 
    ?this lapp:origin ?origin .

    BIND(STRAFTER(str(?origin), "//") AS ?afterScheme)
    BIND(IF(CONTAINS(?afterScheme, "/"), 
            STRBEFORE(?afterScheme, "/"), 
            ?afterScheme) AS ?hostname)
    
    BIND(
      IF(STRENDS(str(?origin), "/"),
         "Origin URL must not end with a trailing slash",
      IF(?hostname = "",
         "Origin URL must have a non-empty hostname",
         "")) AS ?message
    )
    
    FILTER(?message != "")
  }
""" ;
    rdfs:isDefinedBy : .